Proof (finally) that GBI implies GCI

theories/BI.v
@@ -2,14 +2,15 @@ From mathcomp Require Import all_ssreflect.
 Require Import Program.
 From Equations Require Import Equations.
 Require Import extra_principles.
+Require Import continuity_zoo_Prop.
+Require Import Brouwer_ext.
+Require Import brede_herbelin.
 Set Implicit Arguments.
 Unset Strict Implicit.
 Unset Printing Implicit Defensive.
 
 Set Bullet Behavior "Strict Subproofs".
 
-Require Import continuity_zoo_Prop.
-Require Import Brouwer_ext.
 
 Arguments ext_tree {_ _ _}, _ _ _.
 Arguments Btree {_ _}, _ _.
@@ -257,8 +258,6 @@ Proof.
 Qed.
 
 End ContinuousInduction.
-
-
 Section BarInduction.
 
 
@@ -476,3 +475,1844 @@ Proof.
 Qed.
 
 End BarInduction.
+
+Section GeneralisedBarInduction.
+
+Variable I : eqType.
+Variables O A : Type.
+Implicit Type (F : (I -> O) -> A).
+Print GBI.
+Variable HGBI : forall T, @GBI I O T.
+
+Definition is_fun_list (u : seq (I * O)) :=
+  forall i j j', List.In (i, j) u -> List.In (i, j') u -> j = j'.
+
+Lemma is_fun_map (u : seq I) (f : I -> O) :
+  is_fun_list [seq (i, f i) | i <- u].
+Proof.
+  have aux: forall i j, List.In (i, j) [seq (i, f i) | i <- u] -> j = f i.
+  { induction u ; intros i j Hij ; [now inversion Hij | cbn in *].
+    destruct Hij as [Hyp | Hyp] ; [now inversion Hyp | now apply IHu ].
+  }
+  intros i j j' Hj Hj'.
+  apply aux in Hj, Hj' ; now subst.
+Qed.
+
+Lemma is_fun_list_incl (u v : seq (I * O)) :
+  is_fun_list v ->
+  List.incl u v ->
+  is_fun_list u.
+Proof.
+  intros Hfun Hincl i j j' Hin Hin'.
+  apply Hincl in Hin, Hin' ; eapply Hfun ; eassumption.
+Qed.
+
+Lemma is_fun_cat_notin_dom (u v : seq (I * O))
+  (Hu : is_fun_list u)
+  (Hv : is_fun_list v)
+  (Hyp : forall i, ~ (List.In i (map fst u)) \/ ~ (List.In i (map fst v))) :
+  is_fun_list (u ++ v).
+Proof.
+  intros i j j' Hinj Hinj'.
+  specialize (Hyp i) ; destruct Hyp as [Hnotinu | Hnotinv].
+  { suff: List.In (i, j) v.
+    { suff: List.In (i, j') v.
+      { intros Hinv1 Hinv2 ; apply (Hv i) ; assumption. }
+      destruct (List.in_app_or _ _ _ Hinj') ; [ | assumption].
+      exfalso ; apply Hnotinu.
+      now apply (in_map fst) in H ; cbn in H.
+    }
+    destruct (List.in_app_or _ _ _ Hinj) ; [ | assumption].
+    exfalso ; apply Hnotinu.
+    now apply (in_map fst) in H ; cbn in H.
+  }
+  suff: List.In (i, j) u.
+  { suff: List.In (i, j') u.
+    { intros Hinu1 Hinu2 ; apply (Hu i) ; assumption. }
+    destruct (List.in_app_or _ _ _ Hinj') ; [ assumption | ].
+    exfalso ; apply Hnotinv.
+    now apply (in_map fst) in H ; cbn in H.
+  }
+  destruct (List.in_app_or _ _ _ Hinj) ; [ assumption | ].
+  exfalso ; apply Hnotinv.
+  now apply (in_map fst) in H ; cbn in H.
+Qed.
+  
+  
+Lemma is_fun_cons_notin_dom (u : seq (I * O)) (i : I) (o : O)
+  (Hu : is_fun_list u)
+  (H : ~ (List.In i (map fst u))) :
+  is_fun_list ((i,o) :: u).
+Proof.
+  rewrite - cat1s ; apply is_fun_cat_notin_dom ; [ | assumption | ].
+  { intros i' j j' Hinj Hinj' ; cbn in *.
+    destruct Hinj as [Heq | ] ; [ inversion Heq ; subst | now exfalso].
+    destruct Hinj' as [Heq' | ] ; [ inversion Heq' ; now subst | now exfalso].
+  }
+  intros i'.
+  case: (@eqP I i i') ; [intros Heq ; subst ; now right | intros Hnoteq ; left].
+  cbn ; intros [Heq | Hfalse] ; [ now apply Hnoteq | assumption].
+Qed.
+
+Lemma is_fun_rcons_notin_dom (u : seq (I * O)) (i : I) (o : O)
+  (Hu : is_fun_list u)
+  (H : ~ (List.In i (map fst u))) :
+  is_fun_list (rcons u (i,o)).
+Proof.
+  rewrite - cats1 ; apply is_fun_cat_notin_dom ; [ assumption | | ].
+  { intros i' j j' Hinj Hinj' ; cbn in *.
+    destruct Hinj as [Heq | ] ; [ inversion Heq ; subst | now exfalso].
+    destruct Hinj' as [Heq' | ] ; [ inversion Heq' ; now subst | now exfalso].
+  }
+  intros i'.
+  case: (@eqP I i i') ; [intros Heq ; subst ; now left | intros Hnoteq ; right].
+  cbn ; intros [Heq | Hfalse] ; [ now apply Hnoteq | assumption].
+Qed.  
+    
+
+
+Lemma NoDup_rcons {X : Type} (x : X) (l : seq X) :
+  List.NoDup l -> ~ List.In x l -> List.NoDup (rcons l x).
+Proof.
+  induction 1 as [| a l Hnotina k IHk ]; intros Hnotinx.
+  { apply List.NoDup_cons ; [assumption | now econstructor]. }
+  rewrite rcons_cons.
+  econstructor 2.
+  2:{ apply IHk ; intros Hin.
+      apply Hnotinx.
+      now cbn ; right.
+  }
+  rewrite <- cats1 ; intros Hin.
+  apply List.in_app_or in Hin ; destruct Hin as [Hinl | Hinx] ; [now apply Hnotina |].
+  cbn in Hinx ; destruct Hinx as [Heqxq | HFalse] ; [ subst | assumption].
+  apply Hnotinx ; now left.
+Qed.  
+
+Inductive indbarred_fun_list (T : seq (I * O) -> Prop) : seq (I * O) -> Prop :=
+| ieta_fun_list : forall u' u : seq (I * O),
+    T u -> List.incl u u' -> is_fun_list u' -> indbarred_fun_list T u'
+| ibeta_NoDup : forall (a : I) (v : seq (I * O)),
+    ~ List.In a [seq i.1 | i <- v] ->
+    (forall b : O, indbarred_fun_list T (v ++ [:: (a, b)])) ->
+    indbarred_fun_list T v.
+
+
+
+Lemma indbarred_indbarred_fun_list (T : seq (I * O) -> Prop) :
+  indbarred T nil ->
+  indbarred_fun_list T nil.
+Proof.
+  have aux: is_fun_list (@nil (I * O)).
+  { intros q r r' Hin ; now inversion Hin. }
+  revert aux ; generalize (@nil (I * O)) ; intros l Hfun Hyp ; revert Hfun.
+  induction Hyp as [u v Hv Hincl | i v Hnotin k IHk ] ; intros.
+  { econstructor ; eassumption. }
+  econstructor 2 ; [ now apply Hnotin |].
+  intros o ; apply IHk.
+  rewrite cats1 ; apply is_fun_rcons_notin_dom ; assumption.
+Qed.
+
+
+(*Inductive indbarred_NoDup (T : seq (I * O) -> Prop) : seq (I * O) -> Prop :=
+| ieta_NoDup : forall u' u : seq (I * O),
+    T u -> List.incl u u' -> List.NoDup (map fst u') -> indbarred_NoDup T u'
+| ibeta_NoDup : forall (a : I) (v : seq (I * O)),
+    ~ List.In a [seq i.1 | i <- v] ->
+    (forall b : O, indbarred_NoDup T (v ++ [:: (a, b)])) -> indbarred_NoDup T v.
+
+
+
+Lemma indbarred_indbarred_NoDup (T : seq (I * O) -> Prop) :
+  indbarred T nil ->
+  indbarred_NoDup T nil.
+Proof.
+  have aux: List.NoDup (map fst (@nil (I * O))) by (apply List.NoDup_nil).
+  revert aux ; generalize (@nil (I * O)) ; intros l HNoDup Hyp ; revert HNoDup.
+  induction Hyp as [u v Hv Hincl | i v Hnotin k IHk ] ; intros.
+  { econstructor ; eassumption. }
+  econstructor 2 ; [ now apply Hnotin |].
+  intros o ; apply IHk.
+  rewrite cats1.
+  rewrite map_rcons ; apply NoDup_rcons ; cbn ; assumption.
+Qed.
+  
+Lemma indbarred_NoDup_indbarred (T : seq (I * O) -> Prop) :
+  indbarred_NoDup T nil ->
+  indbarred T nil.
+Proof.
+  generalize (@nil (I * O)) ; intros l ; induction 1.
+  { now econstructor ; eassumption. }
+  econstructor 2 ; eassumption.
+Qed.
+*)
+
+
+Fixpoint eval_list (u : seq (I * O)) (i : I) : option O :=
+  match u with
+  | nil => None
+  | (i', o') :: v => if i == i' then Some o' else eval_list v i
+  end.
+
+Fixpoint eval_ext_tree_aux_finapp
+  (tau : @ext_tree I O A) (u: seq (I * O)) (n : nat) (l : seq O)
+  {struct n} : result :=
+  match n with
+  | 0 => tau l
+  | k.+1 =>
+      match tau l with
+      | ask q => match eval_list u q with
+                 | None => ask q
+                 | Some o => eval_ext_tree_aux_finapp tau u k (rcons l o)
+                 end
+      | output _ => tau l
+      end
+  end.
+
+Lemma eval_list_In u i o :
+  eval_list u i = Some o ->
+  List.In (i, o) u.
+Proof.
+  revert i o ; induction u as [ | [i' o'] v IHv] ; intros i o Heq ; cbn in *.
+  { now inversion Heq. }
+  case (@eqP I i i') ; [intros Heqi ; subst ; left | intros Hnoteqi].
+  { erewrite eq_refl in Heq ; inversion Heq  ; now subst. }
+  eapply (introF (b:= i == i') eqP) in Hnoteqi.
+  rewrite Hnoteqi in Heq.
+  apply IHv in Heq ; now right.
+Qed.
+
+  
+Lemma In_eval_list u i o :
+  is_fun_list u ->
+  List.In (i, o) u ->
+  eval_list u i = Some o.
+Proof.
+  revert i o ; induction u as [ | [i' o'] v IHv] ; intros i o Hfun Hin ; cbn in *.
+  { now inversion Hin. }
+  destruct Hin as [Heq | Hin] ; [inversion Heq ; subst ; now rewrite eq_refl | ].
+  case (@eqP I i i') ; [intros Heq ; subst | intros Hnoteq].
+  { f_equal.
+    eapply Hfun ; [left ; reflexivity | now right ].
+  }
+  apply IHv ; [ | assumption].
+  eapply is_fun_list_incl ; [eassumption | ].
+  apply List.incl_tl ; now apply List.incl_refl.
+Qed.
+
+
+Lemma eval_list_In_is_fun u i o :
+  is_fun_list u ->
+  eval_list u i = Some o ->
+  is_fun_list (u ++ [:: (i, o)]).
+Proof.
+  intros Hfun Heq q a a' Hina Hina'. 
+  apply List.in_app_or in Hina, Hina'.
+  destruct Hina as [Hina | Heqa].
+  2:{ destruct Heqa as [Heqa | Hfalse] ; [ inversion Heqa ; clear Heqa ; subst | now inversion Hfalse].
+      destruct Hina' as [Hina' | Heqa']; [ apply In_eval_list in Hina' ; [ | assumption] | ].
+      2:{ destruct Heqa' as [Heqa' | Hfalse] ; [ inversion Heqa' ; now subst | now inversion Hfalse]. }
+      rewrite Heq in Hina' ; now inversion Hina'.
+  }
+  destruct Hina' as [Hina' | Heqa'] ; [eapply Hfun ; now eauto | ].
+  destruct Heqa' as [Heqa' | Hfalse] ; [ inversion Heqa' ; subst | now inversion Hfalse].
+  apply In_eval_list in Hina ; [ | assumption].
+  rewrite Heq in Hina ; now inversion Hina.
+Qed.  
+    
+            
+
+Lemma eval_list_notin u q :
+  eval_list u q = None ->
+  ~ List.In q [seq i.1 | i <- u].
+Proof.
+  revert q ; induction u as [ | [i' o'] v IHv] ; intros i Heq Hin ; [assumption | ].
+  cbn in * ; destruct Hin as [Heq' | Hin] ; [subst | ].
+  { rewrite eq_refl in Heq ; now inversion Heq. }
+  eapply IHv ; [ | eassumption].
+  destruct (i == i') ; [now inversion Heq | assumption].
+Qed.
+
+Lemma eval_list_none_fun u q o :
+  is_fun_list u ->
+  eval_list u q = None ->
+  is_fun_list (u ++ [:: (q,o)]).
+Proof.
+  intros Hfun Hnone ; eapply is_fun_cat_notin_dom ; [assumption | | ].
+  -  intros x y y' [Hyp1 | Hyp1] [Hyp2 | Hyp2] ; inversion Hyp1 ; inversion Hyp2 ; now subst.
+  - intros i.
+    destruct (@eqP I q i) as [Heq | Hnoteq] ; [ subst ; left | ].
+    + now apply eval_list_notin.
+    + cbn ; right ; intros [Hyp | Hyp] ; now auto. 
+Qed.      
+
+
+Lemma eval_list_notin_cat u v q :
+  eval_list u q = None ->
+  ~ List.In q [seq i.1 | i <- v] ->
+  eval_list (u ++ v) q = None.
+Proof.
+  revert q v ; induction u as [ | [i o] u IHu] ; intros q v Heq Hnotin.
+  - cbn.
+    remember (eval_list v q) as aux ; destruct aux as [a | ] ; [ exfalso | reflexivity ].
+    suff: List.In (q, a) v ; [intros Hyp | now apply eval_list_In].
+    apply Hnotin.
+    apply (in_map fst) in Hyp ; now cbn in *.
+  - revert Heq ; cbn ; destruct (q == i) ; [now auto | ].
+    intros Heq ; now eapply IHu ; eauto.
+Qed.
+
+    
+Lemma eval_list_monotone (u v : seq (I * O)) (i : I) (o : O) :
+  is_fun_list v ->
+  List.incl u v ->
+  eval_list u i = Some o ->
+  eval_list v i = Some o.
+Proof.
+  intros Hfun Hincl Heq.
+  apply In_eval_list ; [assumption | ].
+  apply Hincl ; now apply eval_list_In in Heq.
+Qed.
+
+Lemma eval_list_incl_none (u v : seq (I * O)) (i : I):
+  is_fun_list v ->
+  List.incl u v ->
+  eval_list v i = None ->
+  eval_list u i = None.
+Proof.
+  intros Hfun Hincl Heq.
+  remember (eval_list u i) as aux ; destruct aux as [o | ] ; [ | reflexivity].
+  erewrite (eval_list_monotone Hfun Hincl) in Heq ; [eassumption | eauto].
+Qed.
+  
+Lemma eval_ext_tree_aux_finapp_monotone_output_list
+  (tau : @ext_tree I O A) (u v: seq (I * O)) (n : nat) (l : seq O) (a : A) :
+  is_fun_list v ->
+  List.incl u v ->
+  eval_ext_tree_aux_finapp tau u n l = output a ->
+  eval_ext_tree_aux_finapp tau v n l = output a.
+Proof.
+  revert u v l a; induction n as [| k IHk] ; intros * Hfun Hincl Heq ; [assumption| ].
+  cbn in *.
+  remember (tau l) as r ; destruct r as [q | r] ; [ | assumption ].
+  remember (eval_list u q) as ev ; destruct ev as [r' | ] ; [| now inversion Heq ].
+  erewrite eval_list_monotone ; now eauto.
+Qed.
+
+Lemma eval_ext_tree_aux_finapp_monotone_output_fuel
+  (tau : @ext_tree I O A) (u: seq (I * O)) (n k : nat) (l : seq O) (a : A) :
+  eval_ext_tree_aux_finapp tau u n l = output a ->
+  eval_ext_tree_aux_finapp tau u (n + k) l = output a.
+Proof.
+  revert l ; induction n as [ | n IHn] ; cbn in * ; intros l H.
+  1: destruct k ; cbn ; [assumption | now rewrite H].
+  destruct (tau l) ; [ | assumption].
+  destruct (eval_list u s) ; [ | now inversion H].
+  now eapply IHn.
+Qed.
+
+
+Lemma eval_ext_tree_aux_finapp_monotone_ask_list
+  (tau : @ext_tree I O A) (u v: seq (I * O)) (n : nat) (l : seq O) (q : I) :
+  is_fun_list v ->
+  List.incl u v ->
+  eval_list v q = None ->
+  eval_ext_tree_aux_finapp tau u n l = ask q ->
+  eval_ext_tree_aux_finapp tau v n l = ask q.
+Proof.
+  revert u v l q.
+  induction n as [| k IHk] ; intros * Hfun Hincl Hnotin Heq ; [assumption| ].
+  cbn in *.
+  remember (tau l) as r ; destruct r as [q' | r] ; [ | assumption ].
+  remember (eval_list u q') as ev ; destruct ev as [r' | ].
+  - erewrite eval_list_monotone ; now eauto.
+  - injection Heq ; intros Heq' ; subst.
+    remember (eval_list v q) as r' ; destruct r' as [q' | ] ; [ | reflexivity].
+    symmetry in Heqr' ; apply eval_list_In, (in_map fst) in Heqr'.
+    exfalso ; now inversion Hnotin.
+Qed.
+
+
+Lemma eval_ext_tree_aux_finapp_monotone_ask_list_nomorefuel
+  (tau : @ext_tree I O A) (u v: seq (I * O)) (n : nat) (l : seq O) (q : I) (a : O) :
+  is_fun_list v ->
+  List.incl u v ->
+  eval_list u q = Some a ->
+  eval_ext_tree_aux_finapp tau u n l = ask q ->
+  eval_ext_tree_aux_finapp tau v n l = ask q.
+Proof.
+  revert u v l q.
+  induction n as [| k IHk] ; intros * Hfun Hincl Hnotin Heq ; [assumption| ].
+  cbn in *.
+  remember (tau l) as r ; destruct r as [q' | r] ; [ | assumption ].
+  remember (eval_list u q') as ev ; destruct ev as [r' | ].
+  - erewrite eval_list_monotone ; now eauto.
+  - injection Heq ; intros Heq' ; subst.
+    rewrite Hnotin in Heqev ; now inversion Heqev.
+Qed.
+
+Lemma eval_ext_tree_aux_finapp_monotone_ask_fuel
+  (tau : @ext_tree I O A) (u : seq (I * O)) (n m : nat) (l : seq O) (q : I) :
+  is_fun_list u ->
+  eval_list u q = None ->
+  eval_ext_tree_aux_finapp tau u n l = ask q ->
+  eval_ext_tree_aux_finapp tau u (n + m) l = ask q.
+Proof.
+  revert u n l q.
+  induction n as [| k IHk] ; intros * Hfun Hnotin Heq ; cbn in *.
+  - destruct m ; cbn ; [ assumption | now rewrite Heq Hnotin ].
+  - destruct (tau l) ; cbn in * ; [ | now inversion Heq ].
+    destruct (eval_list u s) ; cbn in * ; [ | assumption].
+    now apply IHk.
+Qed.
+
+Lemma eval_ext_tree_aux_finapp_one_step_fuel tau u v w l n q a :
+  is_fun_list v ->
+  is_fun_list w ->
+  List.incl u v ->
+  List.incl u w ->
+  eval_list u q = Some a ->
+  eval_ext_tree_aux_finapp tau u n l = ask q ->
+  eval_ext_tree_aux_finapp tau v n.+1 l = eval_ext_tree_aux_finapp tau w n.+1 l.
+Proof.
+  revert u v w l q.
+  induction n as [ | n IHn] ; intros * Hfunv Hfunw Hinclv Hinclw Heval Hasku.
+  - cbn in *.
+    rewrite Hasku.
+    now do 2 (erewrite eval_list_monotone ; eauto).
+  - cbn in *.
+    remember (tau l) as aux ; destruct aux as [i | r] ; subst ; [ | now inversion Hasku].
+    remember (eval_list u i) as aux2 ; destruct aux2 as [ o | ].
+    2:{ inversion Hasku ; subst.
+        rewrite Heval in Heqaux2 ; now inversion Heqaux2.
+    }
+    now do 2 (erewrite eval_list_monotone ; eauto).
+Qed.
+
+Print indbarred_fun_list.
+
+Inductive indbarred_ext_tree (T : seq (I * O) -> Prop) (tau : ext_tree) :
+  seq (I * O) -> Prop :=
+|  ieta_ext_tree : forall (u' u : seq (I * O)) (r : A),
+    T u ->
+    List.incl u u' ->
+    is_fun_list u' ->
+    eval_ext_tree_aux_finapp tau u (size u) nil = output r ->
+    eval_ext_tree_aux_finapp tau u' (size u') nil = output r ->
+    indbarred_ext_tree T tau u'
+| isucc_ext_tree : forall (u : seq (I * O)) (q : I) (a : O),
+    is_fun_list u ->
+    eval_ext_tree_aux_finapp tau u (size u) nil = ask q ->
+    eval_list u q = Some a ->
+    indbarred_ext_tree T tau (u ++[:: (q, a)]) ->
+    indbarred_ext_tree T tau u
+| ibeta_ext_tree : forall (u : seq (I * O)) (q : I),
+    is_fun_list u ->
+    eval_ext_tree_aux_finapp tau u (size u) nil = ask q ->
+    eval_list u q = None ->
+    (forall o : O, indbarred_ext_tree T tau (u ++ [:: (q, o)])) ->
+    indbarred_ext_tree T tau u.
+
+
+Print Acc.
+
+Inductive goodRel (tau : ext_tree) : seq (I * O) -> seq (I *O) -> Prop :=
+| goodRel_in_dom u i i' o : is_fun_list u ->
+                          eval_ext_tree_aux_finapp tau u (size u) nil = ask i ->
+                          eval_list u i' = None ->
+                          goodRel tau (u ++ [:: (i', o)]) u
+| goodRel_notin_dom u i i' o : is_fun_list u ->
+                             eval_ext_tree_aux_finapp tau u (size u) nil = ask i ->
+                             eval_list u i' = Some o ->
+                             goodRel tau (u ++ [:: (i', o)]) u.
+
+Lemma hope (tau : ext_tree) (l : seq (I * O)) :
+  indbarred_fun_list
+    (fun u => exists n a, eval_ext_tree_aux_finapp tau u n nil = output a) l ->
+  Acc (goodRel tau) l.
+Proof.
+  induction 1 as [v u [n [r Hr]] Hincl Hfun | q v Hnotin _ IHk] ; intros.
+  - have aux := eval_ext_tree_aux_finapp_monotone_output_list Hfun Hincl Hr.
+    clear u Hr Hincl.
+    case (leqP n (size v)).
+    { apply (eval_ext_tree_aux_finapp_monotone_output_fuel (size v - n)) in aux.
+      intros Hinf ; apply subnK in Hinf.
+      rewrite addnC in Hinf ; rewrite Hinf in aux.
+      econstructor ; intros u Hu.
+      destruct Hu as [u i i' o Hfunu Hask Hnone | u i i' o Hfunu Hask Hsome ].
+      1,2: rewrite aux in Hask ; now inversion Hask.
+    }
+    intros Hinf ; apply leqW in Hinf ; cbn in Hinf ; apply subnK in Hinf.
+    rewrite addnC in Hinf ; rewrite - Hinf in aux.
+    clear Hinf ; revert r Hfun aux.
+    generalize (n - size v) as k ; intros k ; clear n ; revert v.
+    induction k as [ | k IHk].
+    + intros.
+      rewrite addn0 in aux.
+      econstructor ; intros u Hu.
+      destruct Hu as [ u i i' o Hfunu Hask Hnone | u i i' o Hfunu Hask Hsome ].
+      1,2 : rewrite aux in Hask ; now inversion Hask.
+    + intros.
+      econstructor ; intros u Hu.
+      destruct Hu as [u i i' o Hfunu Hask Hnone | u i i' o Hfunu Hask Hsome ].
+      * apply (IHk _ r) ; [now apply eval_list_none_fun | ].
+        rewrite size_cat addn1 addSn - addnS.
+        unshelve eapply (eval_ext_tree_aux_finapp_monotone_output_list _ _ aux).
+        -- now apply eval_list_none_fun.
+        -- now apply List.incl_appl, List.incl_refl.
+      * apply (IHk _ r) ; [ now apply eval_list_In_is_fun | ].
+        rewrite size_cat addn1 addSn - addnS.
+        unshelve eapply (eval_ext_tree_aux_finapp_monotone_output_list _ _ aux).
+        -- now apply eval_list_In_is_fun.
+        -- now apply List.incl_appl, List.incl_refl.
+  - econstructor ; intros u Hu.
+    destruct Hu as [u i i' o Hfunu Hask Hnone | u i i' o Hfunu Hask Hsome ].
+Abort.
+
+Unset Elimination Schemes.
+
+Inductive ext_tree_indbarredP (tau : ext_tree) (l: seq (I * O)) : Prop :=
+| etree_in : is_fun_list l ->
+             ((exists q, eval_ext_tree_aux_finapp tau l (size l) nil = ask q /\
+                           eval_list l q = None /\
+                           (forall a, ext_tree_indbarredP tau (l ++ [:: (q,a)]))) \/
+                
+                (exists r, eval_ext_tree_aux_finapp tau l (size l) nil = output r) \/
+                
+                (exists q a, eval_ext_tree_aux_finapp tau l (size l) nil = ask q /\
+                             eval_list l q = Some a /\
+                             ext_tree_indbarredP tau (l ++ [:: (q, a)]))) ->
+             ext_tree_indbarredP tau l.
+
+Set Elimination Schemes.
+
+Inductive ext_tree_indbarred (tau : ext_tree) (l : seq (I * O)) : Type :=
+| ext_tree_eta r : is_fun_list l ->
+                   eval_ext_tree_aux_finapp tau l (size l) nil = output r ->
+                   ext_tree_indbarred tau l
+| ext_tree_succ q a : is_fun_list l ->
+                      eval_ext_tree_aux_finapp tau l (size l) nil = ask q ->
+                      eval_list l q = Some a ->
+                      ext_tree_indbarred tau (l ++ [:: (q, a)]) ->
+                      ext_tree_indbarred tau l
+| ext_tree_beta q : is_fun_list l ->
+                    eval_ext_tree_aux_finapp tau l (size l) nil = ask q ->
+                    eval_list l q = None ->
+                    (forall a, ext_tree_indbarred tau (l ++ [:: (q,a)])) ->
+                      ext_tree_indbarred tau l.
+
+(* econstructor ; [assumption | ].
+    right ; left ; exists r.
+    eapply eval_ext_tree_aux_finapp_monotone_output_list ; now eauto.
+  - econstructor ; [assumption | ].
+    right ; right.
+    exists q, a ; split ; [ | split ; [eapply eval_list_monotone ; eassumption | ] ].
+    2:{ eapply ext_tree_indbarredP_monotone_list ; now eauto. }
+    eapply eval_ext_tree_aux_finapp_monotone_ask_list_nomorefuel ; now eauto.
+Defined.    *)
+
+Fixpoint ext_tree_indbarredP_rect
+  (tau : ext_tree)
+  (P : seq (I * O) -> Type)
+  (Hout : forall (l : seq (I * O)) (r : A) (Hfun : is_fun_list l)
+                 (e : eval_ext_tree_aux_finapp tau l (size l) [::] = output r), 
+      P l)
+  (Hsucc : forall (l : seq (I * O)) (q : I) (a : O) (Hfun : is_fun_list l)
+                 (Heq : eval_ext_tree_aux_finapp tau l (size l) [::] = ask q)
+                 (Hnone : eval_list l q = Some a)
+                 (e : ext_tree_indbarredP tau (l ++ [:: (q, a)])),
+      P (l ++ [:: (q,a) ]) -> P l)
+  (Hask : forall (l : seq (I * O)) (q : I) (Hfun : is_fun_list l)
+                 (Heq : eval_ext_tree_aux_finapp tau l (size l) [::] = ask q)
+                 (Hnone : eval_list l q = None)
+                 (e : forall a : O, ext_tree_indbarredP tau (l ++ [:: (q,a)])),
+      (forall a : O, P (l ++ [:: (q,a)])) -> P l)
+  (l : seq (I * O)) (e : ext_tree_indbarredP tau l) : P l.
+Proof.
+  destruct e as [Hnodup Hq].
+  remember (eval_ext_tree_aux_finapp tau l (size l) [::]) as aux.
+  destruct aux as [q | r].
+  - remember (eval_list l q) as aux2 ; destruct aux2 as [a | ].
+    + suff: ext_tree_indbarredP tau (l ++ [:: (q, a)]).
+      { intros Hyp ; eapply Hsucc ; eauto. 
+        now apply (ext_tree_indbarredP_rect tau P Hout Hsucc Hask).
+      }
+      destruct Hq as [[q' [Heq [Hnone Hq']]] | [[r Hr] | [q' [a' [Heq' [Hq' IH]]]]]] ; [ | now inversion Hr |  ].
+      * injection Heq ; intros Heqq ; subst.
+        rewrite Hnone in Heqaux2 ; now inversion Heqaux2.
+      * inversion Heq' ; subst.
+        rewrite Hq' in Heqaux2 ; inversion Heqaux2 ; now subst.
+    + suff: forall a : O, ext_tree_indbarredP tau (l ++ [:: (q, a)]).
+      { intros Hyp.
+        eapply (Hask l q Hnodup) ; [now auto | now symmetry | assumption | ] ; intros a.
+        apply (ext_tree_indbarredP_rect tau P Hout Hsucc Hask) ; now apply Hyp.
+      }
+      destruct Hq as [[q' [Heq' Ho]]| [[r Hr] | [q' [a' [Heval [Hsome Hsuc]]]]]] ; [| now inversion Hr | ].
+      * inversion Heq' ; subst ; now eapply Ho.
+      * exfalso.
+        injection Heval ; intros Heq ; subst.
+        rewrite Hsome in Heqaux2 ; now inversion Heqaux2.
+  - eapply (Hout l r Hnodup).
+    destruct Hq as [[q [Heq Ho]]| [[r' Hr] | [q' [a' [Heval _]]]]] ; [ now inversion Heq | | now inversion Heval ].
+    inversion Hr ; now subst.
+Defined.
+
+
+Lemma ext_tree_indbarredP_ind
+  (tau : ext_tree)
+  (P : seq (I * O) -> Prop)
+  (Hout : forall (l : seq (I * O)) (r : A) (Hfun : is_fun_list l)
+                 (e : eval_ext_tree_aux_finapp tau l (size l) [::] = output r), 
+      P l)
+  (Hsucc : forall (l : seq (I * O)) (q : I) (a : O) (Hfun : is_fun_list l)
+                 (Heq : eval_ext_tree_aux_finapp tau l (size l) [::] = ask q)
+                 (Hnone : eval_list l q = Some a)
+                 (e : ext_tree_indbarredP tau (l ++ [:: (q, a)])),
+      P (l ++ [:: (q,a) ]) -> P l)
+  (Hask : forall (l : seq (I * O)) (q : I) (Hfun : is_fun_list l)
+                 (Heq : eval_ext_tree_aux_finapp tau l (size l) [::] = ask q)
+                 (Hnone : eval_list l q = None)
+                 (e : forall a : O, ext_tree_indbarredP tau (l ++ [:: (q,a)])),
+      (forall a : O, P (l ++ [:: (q,a)])) -> P l)
+  (l : seq (I * O)) (e : ext_tree_indbarredP tau l) : P l.
+Proof.
+  eapply ext_tree_indbarredP_rect ; eauto.
+Qed.  
+
+
+
+(*
+  (tau : ext_tree)
+  (P : forall l : seq (I * O), Type)
+       (Hyp : forall (l : seq (I * O)) (q : I) (n : List.NoDup [seq i.1 | i <- l])
+          (e : eval_ext_tree_aux_finapp tau l (size l) [::] = ask q)
+          (e0 : forall a : O, ext_tree_indbarredP tau ((q, a) :: l)),
+        (forall a : O, P ((q, a) :: l)) -> P l)
+        (l : seq (I * O)) (e : ext_tree_indbarredP tau l) : P l.
+Proof.
+  destruct e as [Hnodup Hq].
+  remember (eval_ext_tree_aux_finapp tau l (size l) [::]) as aux.
+  destruct aux as [q | r].
+  - eapply (Hyp l q Hnodup) ; [now auto | | ] ; intros a.
+    + destruct Hq as [q' [Heq' Ho]] ; inversion Heq' ; subst.
+      now eapply Ho.
+    + apply (ext_tree_indbarredP_rect tau P Hyp).
+      destruct Hq as [q' [Heq' Ho]] ; inversion Heq' ; subst.
+      now apply Ho.
+  - exfalso.
+    destruct Hq as [q' [Heq' Ho]].
+    now inversion Heq'.
+Defined.
+*)
+Lemma ext_tree_indbarred_spec (tau : ext_tree) (l : seq (I * O)) (n : nat) :
+  ext_tree_indbarredP tau l ->
+  ext_tree_indbarred tau l.
+Proof.
+  induction 1 as [l a Hnodup Heqa | l q Hnodup Heq ? IHk  | Hsuc].
+  - econstructor 1 ; eassumption.
+  - econstructor 2 ; eauto. 
+  - econstructor 3 ; now eauto.
+Qed.
+
+Lemma ext_tree_indbarred_dialogue
+  (tau : ext_tree) (Hvalid : valid_ext_tree tau)
+  (Hyp : ext_tree_indbarred tau nil) :
+  {d : dialogue & forall alpha, exists n, eval_ext_tree tau alpha n = output (deval d alpha)}.
+Proof.
+  unfold eval_ext_tree.
+  revert Hyp ; generalize (@nil (I * O)).
+  intros l Hyp ; pattern l.
+  induction Hyp.
+  - exists (eta r).
+    intros alpha ; exists (size l).
+    cbn in *.
+    admit.
+  - assumption.
+  - destruct l as [ | [q' o'] v].
+    + cbn in *.
+      exists (beta q (fun o => projT1 (X o))).
+      intros alpha.
+      destruct (projT2 (X (alpha q)) alpha) as [n Hn].
+      exists n.
+      now cbn.
+    + exact (X o').
+Admitted
+              .
+(*Lemma indbarred_NoDup_NoDup T l:
+  indbarred_NoDup T l ->
+  List.NoDup (map fst l).
+Proof.
+  induction 1 as [ | q v Hnotin k IHk] ; [ assumption | ].
+  destruct v as [ | [q' a] v] ; [now econstructor | ].
+  specialize (IHk a).
+  rewrite map_cat in IHk.
+  now apply List.NoDup_remove_1 in IHk ; rewrite -> cats0 in IHk.
+Qed.
+ *)
+
+Lemma eval_output_indbarredP tau u n r :
+  is_fun_list u ->
+  eval_ext_tree_aux_finapp tau u n nil = output r ->
+  ext_tree_indbarredP tau u.
+Proof.
+  intros Hfun Hyp.
+  case: (leqP n (size u)) ; intros Hinf.
+  - apply subnKC in Hinf.
+    econstructor ; [assumption | right ; left ].
+    exists r ; rewrite - Hinf.
+    now apply eval_ext_tree_aux_finapp_monotone_output_fuel.
+  - apply leqW in Hinf ; cbn in Hinf ; apply subnKC in Hinf.
+    remember (eval_ext_tree_aux_finapp tau u (size u) [::]) as aux ; destruct aux as [q | r'].
+    2: econstructor ; [assumption | right ; left ; now exists r'].
+    remember (eval_list u q) as aux2 ; destruct aux2 as [ a | ].
+    2:{ symmetry in Heqaux ; eapply (eval_ext_tree_aux_finapp_monotone_ask_fuel (n - size u)) in Heqaux ; eauto.
+        rewrite Hinf Hyp in Heqaux ; now inversion Heqaux.
+    }
+    remember (n - size u) as m ; clear Heqm.
+    revert n q a u Hfun Hyp Hinf Heqaux Heqaux2 ; induction m as [ | k IHk] ; intros.
+    + erewrite <- plus_n_O in Hinf ; subst ; exfalso.
+      rewrite Hyp in Heqaux ; now inversion Heqaux.
+    + econstructor ; [assumption | ].
+      right ; right.
+      exists q,a ; split ; [now auto | split ; [now auto | ] ].
+      remember (eval_ext_tree_aux_finapp tau (u ++ [:: (q, a)]) (size u + 1) [::]) as aux3.
+      destruct aux3 as [q' | r'].
+      2:{ econstructor ; [ now apply eval_list_In_is_fun | ].
+          right ; left ; exists r' ; now rewrite size_cat. }
+      remember (eval_list u q') as aux4.
+      destruct aux4 as [a' | ].
+      { apply (IHk n q' a') ; eauto.
+        * now apply eval_list_In_is_fun.
+        * eapply eval_ext_tree_aux_finapp_monotone_output_list ;
+            [ now apply eval_list_In_is_fun | | eassumption ].
+          now apply List.incl_appl, List.incl_refl.
+        * now rewrite <- Hinf, size_cat, <- plus_n_Sm, addn1, plus_Sn_m.
+        * now rewrite size_cat.
+        * symmetry ; eapply eval_list_monotone ; eauto ; [ now apply eval_list_In_is_fun | ].
+          now apply List.incl_appl, List.incl_refl.
+      }
+      exfalso.
+      rewrite <- Hinf, <- plus_n_Sm, <- plus_Sn_m in Hyp.
+      erewrite eval_ext_tree_aux_finapp_monotone_ask_fuel in Hyp ; eauto ; [now inversion Hyp | ].
+      eapply eval_ext_tree_aux_finapp_monotone_ask_list ; eauto ; [ | now rewrite Heqaux3 addn1].
+      apply List.incl_app ; [now apply List.incl_refl | ].
+      intros [x y] [Hin | Hfalse] ; [ inversion Hin ; subst | now eauto].
+      now apply eval_list_In.
+Qed.      
+
+
+Lemma indbarred_fun_list_fun_list T l:
+  indbarred_fun_list T l ->
+  is_fun_list l.
+Proof.
+  induction 1 as [ | q v Hnotin k IHk] ; [ assumption | ].
+  destruct v as [ | [q' a] v];  [intros ??? Hin ; now inversion Hin | ].
+  specialize (IHk a).
+  eapply is_fun_list_incl ; [eassumption | ].
+  now apply List.incl_appl, List.incl_refl.
+Qed.
+
+
+Fixpoint ext_tree_indbarredP_monotone tau u v
+  (Hu : ext_tree_indbarredP tau u) {struct Hu}:
+  is_fun_list v ->
+  List.incl u v ->
+  ext_tree_indbarredP tau v.
+Proof.
+  intros Hfunv Hincl.
+  destruct Hu as [Hfunu Hyp].
+  destruct Hyp as [[q [Heq [Hnone Hq]]]| [[r Hr] | [q [a [Heval [Hsome Hsuc]]]]]].
+  - remember (eval_list v q) as aux ; destruct aux as [ a | ].
+    + apply (ext_tree_indbarredP_monotone tau _ _ (Hq a) Hfunv).
+      apply List.incl_app ; [assumption | ].
+      intros [q' o'] [Hyp | Hyp] ; inversion Hyp; subst.
+      now apply eval_list_In.
+    + suff: forall (a : O) w, List.incl (v ++ [:: (q, a)]) w ->
+                              is_fun_list w ->
+                              ext_tree_indbarredP tau w.
+      2:{ intros a w Hincl' Hfun' ; apply (ext_tree_indbarredP_monotone tau _ _ (Hq a) Hfun').
+          eapply List.incl_tran ; [ | eassumption].
+          apply List.incl_app ; [now apply List.incl_appl | apply List.incl_appr].
+          now apply List.incl_refl.
+      }
+      intros Hyp.
+      case: (leqP (size u) (size v)) ; intros Hinf.
+      * apply subnKC in Hinf.
+        econstructor ; [assumption | ].
+        left ; exists q ; split ; [ | split ; [now auto | ] ].
+        2:{ intros a ; apply (Hyp a) ; [now apply List.incl_refl | ].
+            rewrite cats1 ; apply is_fun_rcons_notin_dom ; [assumption | ].
+            now apply eval_list_notin.
+        }
+        rewrite - Hinf.
+        erewrite (eval_ext_tree_aux_finapp_monotone_ask_fuel (size v - size u)) ; eauto.
+        eapply eval_ext_tree_aux_finapp_monotone_ask_list ; now eauto.
+      * apply leqW in Hinf ; cbn in Hinf ; apply subnKC in Hinf ; rewrite - Hinf in Heq.
+        remember (size u - size v) as n ; clear Heqn.
+        revert u v Hinf Hincl Hfunu Hfunv Hnone Hq Heq Heqaux Hyp.
+        induction n ; cbn ; intros.
+        { rewrite <- plus_n_O in Hinf, Heq.
+          econstructor ; [assumption | ].
+          left ; exists q ; split ;
+            [now eapply eval_ext_tree_aux_finapp_monotone_ask_list ; eauto | ].
+          split ; [now eauto | ].
+          intros a ; apply (Hyp a) ; [now apply List.incl_refl | ].
+          rewrite cats1 ; apply is_fun_rcons_notin_dom ; [assumption | ].
+          now apply eval_list_notin.
+        }
+        remember (eval_ext_tree_aux_finapp tau v (size v) [::]) as auxv ; destruct auxv as [q' | ].
+        2:{ eapply eval_ext_tree_aux_finapp_monotone_ask_list in Heq ; eauto.
+            symmetry in Heqauxv.
+            eapply (eval_ext_tree_aux_finapp_monotone_output_fuel n.+1) in Heqauxv ; eauto.
+            rewrite Heq in Heqauxv ; now inversion Heqauxv.
+        }
+        case: (@eqP I q q') ; [intros Heqq ; subst | intros Hnoteq].
+        -- econstructor ; [assumption | ].
+           left ; exists q' ; split ; [now auto | split ; [now trivial | ]].
+           intros a ; apply (Hyp a) ; [now apply List.incl_refl | ].
+           rewrite cats1 ; apply is_fun_rcons_notin_dom ; [assumption | ].
+           now apply eval_list_notin.
+        -- econstructor ; [assumption | ].
+           remember (eval_list v q') as auxv ; destruct auxv as [ a| ].
+           { right ; right.
+             exists q', a ; split ; [now auto | split ; [now auto | ] ].
+             apply (IHn u) ; eauto.
+             ++ rewrite size_cat ; cbn ; now rewrite -> addn1, plus_Sn_m, plus_n_Sm.
+             ++ now apply List.incl_appl.
+             ++ now apply eval_list_In_is_fun.
+             ++ now rewrite size_cat ; cbn ; rewrite -> addn1, plus_Sn_m, plus_n_Sm.
+             ++ symmetry ; apply eval_list_notin_cat ; [now auto | cbn].
+                intros [Heq' | Hfalse] ; [ subst | now inversion Hfalse].
+                now apply Hnoteq.
+             ++ intros a' w Hincl' Hfunw.
+                apply (Hyp a') ; [ | assumption].
+                eapply List.incl_tran ; [ | eassumption].
+                apply List.incl_app ; [do 2 apply List.incl_appl ; now apply List.incl_refl | ].
+                now apply List.incl_appr, List.incl_refl.
+           }
+           left.
+           exists q' ; split ; [now auto | split ; [now auto | ] ].
+           intros a.
+           eapply (IHn u) ; eauto.
+           ++ rewrite size_cat ; cbn ; now rewrite -> addn1, plus_Sn_m, plus_n_Sm.
+           ++ now apply List.incl_appl.
+           ++ rewrite cats1 ; apply is_fun_rcons_notin_dom ; [assumption | ].
+              now apply eval_list_notin.
+           ++ now rewrite <- Heq, size_cat, <- plus_n_Sm, <- plus_Sn_m, addn1.
+           ++ symmetry ; apply eval_list_notin_cat ; [now auto | cbn].
+              intros [Heq' | Hfalse] ; [ subst | now inversion Hfalse].
+              now apply Hnoteq.
+           ++ intros a' w Hincl' Hfunw.
+              apply (Hyp a') ; [ | assumption].
+              eapply List.incl_tran ; [ | eassumption].
+              apply List.incl_app ; [do 2 apply List.incl_appl ; now apply List.incl_refl | ].
+              now apply List.incl_appr, List.incl_refl.
+  - eapply eval_output_indbarredP ; [eassumption | ].
+    eapply eval_ext_tree_aux_finapp_monotone_output_list ; eassumption.
+  - apply (ext_tree_indbarredP_monotone _ _ _ Hsuc Hfunv).
+    apply List.incl_app ; [assumption | ].
+    intros [x y] [Hin | Hfalse] ; [ inversion Hin ; subst | now inversion Hfalse].
+    now apply Hincl, eval_list_In.
+Defined.    
+
+Print eval_ext_tree_aux_finapp.
+
+Fixpoint eval_ext_tree_aux_finapp_minimal_list
+  (tau : ext_tree (R := A)) (u : seq (I * O)) (n : nat) (l : seq O) {struct n} :
+    seq (I * O) :=
+  match n, tau l with
+  | 0, _ => [::]
+  | _, output _ => [::]
+  | k.+1, ask q => match eval_list u q with
+                   | None => [::]
+                   | Some o => (q, o) :: eval_ext_tree_aux_finapp_minimal_list tau u k (rcons l o)
+                   end
+  end.
+
+Print List.Add.
+
+Lemma Add_rcons {X : Type} (a : X) (l : seq X): List.Add a l (rcons l a).
+Admitted.
+
+Lemma Add_cat {X : Type} (a : X) (u v w : seq X) :
+  List.Add a u v ->
+  List.Add a (u ++ w) (v ++ w).
+Admitted.
+
+Lemma Add_diamond {X : Type} (x y : X) (u v w l : seq X) :
+  List.Add x u v -> List.Add y v l -> List.Add x w l -> List.Add y u w.
+Admitted.
+
+
+Lemma super (tau : ext_tree) (u v : seq (I * O)) (i : I) (o : O) :
+  eval_list u i = None ->
+  List.Add (i,o) u v ->
+  (ext_tree_indbarredP tau v) ->
+  (forall a w, List.Add (i, a) u w ->
+               ext_tree_indbarredP tau w) ->
+  ext_tree_indbarredP tau u.
+Proof.
+  intros Hnone Hadd Hv Hyp.
+  have Hincl : List.incl u v.
+  { intros x Hin ; eapply List.Add_in ; [eassumption | now right]. }
+  revert u Hincl Hnone Hadd Hyp.
+  induction Hv as [l a Hnodup Heqa | l q o' Hfunl Heq Hsome k IHk |
+                    l q Hfunl Heq Hnonel k IHk] ; intros.
+  - have Hfunu : is_fun_list u.
+    { eapply is_fun_list_incl ; eassumption. } 
+    have Heq: (size l = (size u).+1) by (eapply List.Add_length ; eassumption).
+    rewrite Heq in Heqa.
+    remember (eval_ext_tree_aux_finapp tau u (size u) nil) as aux.
+    destruct aux as [q' | r].
+    2: econstructor ; [ assumption | right ; left ; now exists r].
+    remember (eval_list u q') as aux2 ; destruct aux2 as [a' | ].
+    + econstructor ; [assumption | right ; right ; exists q', a' ].
+      split ; [now auto | split ; [now auto | ] ].
+      remember (eval_ext_tree_aux_finapp tau (u ++ [:: (q', a')]) (size u).+1 [::])
+        as aux3.
+      destruct aux3 as [q'' | r'].
+      2:{ econstructor ; [ now apply eval_list_In_is_fun | ].
+          right ; left ; exists r' ; now rewrite size_cat addn1.
+      }
+      econstructor ; [now apply eval_list_In_is_fun | right ; left ].
+      exists a ; rewrite size_cat addn1 - Heqa.
+      eapply (eval_ext_tree_aux_finapp_one_step_fuel) ; eauto.
+      * now apply eval_list_In_is_fun.
+      * now apply List.incl_appl, List.incl_refl.
+    + destruct (@eqP I q' i) as [Heq' | Hnoteq] ; [subst | ].
+      * econstructor ; [assumption | ].
+        left ; exists i ; split ; [auto | split ; [assumption | ] ].
+        intros a' ; apply (Hyp a').
+        rewrite cats1 ; now apply Add_rcons.
+      * exfalso.
+        suff: eval_ext_tree_aux_finapp tau l (size u).+1 [::] = ask q'.
+        {intros Heq' ; rewrite Heq' in Heqa ; now inversion Heqa. }
+        suff: eval_list l q' = None.
+        { intros Hnonel.
+          rewrite - addn1 ; apply eval_ext_tree_aux_finapp_monotone_ask_fuel ; auto .
+          now eapply eval_ext_tree_aux_finapp_monotone_ask_list ; eauto.
+        }
+        suff: eval_list (u ++ [::(i,o)]) q' = None.
+        { intros Hnoneu.
+          eapply eval_list_incl_none with (u ++ [:: (i, o)]) ; eauto.
+          * now apply eval_list_none_fun.
+          * intros x Hinx.
+            eapply (List.Add_in Hadd) in Hinx.
+            destruct Hinx as [Hl | Hr] ; apply List.in_or_app ; [right | ] ; now left.
+        }
+        apply eval_list_notin_cat ; [now auto | cbn].
+        intros [Heqi | Hfalse] ; auto.
+  - have Hfunu : is_fun_list u by (eapply is_fun_list_incl ; eassumption).
+    have Heqsize : size l = (size u).+1 by (eapply List.Add_length ; eassumption).
+    rewrite Heqsize in Heq.
+    remember (eval_ext_tree_aux_finapp tau u (size u) nil) as aux.
+    destruct aux as [q' | r].
+    2: econstructor ; [ auto | right ; left ; now exists r ].
+    remember (eval_list u q') as aux2 ; destruct aux2 as [a | ].
+    + econstructor ; [ auto | ].
+      right ; right ; exists q',a.
+      split ; [now auto | split ; [now auto | ] ].
+      remember (eval_ext_tree_aux_finapp tau (u ++[:: (q', a)]) (size (u ++ [:: (q', a)])) nil)
+        as aux3.
+      destruct aux3 as [q'' | r].
+      2: econstructor ; [ now apply eval_list_In_is_fun | right ; left ; now exists r ].
+      suff: q'' = q.
+      2:{ suff: ask (R:= A) q'' = ask q ; [ intros H ; now inversion H | ].
+          rewrite Heqaux3 - Heq size_cat addn1.
+          erewrite (eval_ext_tree_aux_finapp_one_step_fuel (u := u) (v := l)) ; eauto.
+          * now apply eval_list_In_is_fun.
+          * apply List.incl_appl, List.incl_refl.
+      }
+      intros H ; subst.
+      remember (eval_list u q) as aux4 ; destruct aux4 as [a' | ].
+      * have auxeq : o' = a'.
+        { suff : Some o' = Some a' by (intros H ; now inversion H).
+          rewrite - Hsome ; eapply eval_list_monotone ; eauto.
+        }
+        subst.
+        have auxeval : eval_list (u ++ [:: (q', a)]) q = Some a'.
+        { eapply eval_list_monotone with u ; [now apply eval_list_In_is_fun | | eauto ].
+          now apply List.incl_appl, List.incl_refl.
+        }
+        econstructor ; [now apply eval_list_In_is_fun | right ; right ].
+        exists q, a' ; split ; [auto | split ; [ auto | ] ].
+        suff: ext_tree_indbarredP tau (u ++ [::(q,a')]).
+        { intros H ; apply (ext_tree_indbarredP_monotone H).
+          + apply eval_list_In_is_fun ; [ now apply eval_list_In_is_fun | auto ].
+          + apply List.incl_app ; [ | now apply List.incl_appr, List.incl_refl].
+            do 2 apply List.incl_appl ; now apply List.incl_refl.
+        }
+        destruct (@eqP I i q) as [e | n] ; [ subst | ].
+        { rewrite - Heqaux4 in Hnone ; now inversion Hnone. }
+        unshelve eapply IHk.
+        -- apply List.incl_app ; [now apply List.incl_appl | ].
+           apply List.incl_appr, List.incl_refl.
+        -- apply eval_list_notin_cat ; [assumption | ].
+           cbn ; intros [Hfalse | Hfalse] ; [ | now inversion Hfalse].
+           now apply n.
+        -- now apply Add_cat.
+        -- intros o' w Haddw.
+           suff: ext_tree_indbarredP tau (u ++ [::(i, o')]).
+           { intros H ; unshelve eapply (ext_tree_indbarredP_monotone H).
+             + eapply is_fun_list_incl with ((u ++ [:: (q, a')]) ++ [::(i, o')]).
+               { apply eval_list_none_fun ; [ now apply eval_list_In_is_fun | ].
+                 eapply eval_list_incl_none with u ; eauto.
+                 apply List.incl_app ; [now apply List.incl_refl | ].
+                 apply List.incl_cons ; [ | now apply List.incl_nil_l].
+                 now apply eval_list_In.
+               }
+               intros y Hiny ; apply (List.Add_in Haddw) in Hiny.
+               destruct Hiny as [Hiny | Hiny] ; [subst | ].
+               ++ apply List.in_or_app ; right ; now left.
+               ++ apply List.in_or_app ; now left.
+             + intros x Hin ; eapply List.Add_in ; [eassumption | ].
+               destruct (List.in_app_or _ _ _ Hin) as [Hin2 | Hin2] ; [right | ].
+               * now apply List.in_or_app ; left.
+               * destruct Hin2 as [Hin2 | Hin2] ; inversion Hin2 ; now left.
+           }
+           eapply (Hyp o').
+           rewrite <- cat1s, <- (cats0 u) at 1.
+           apply List.Add_app.
+      * have auxeval : eval_list (u ++ [:: (q', a)]) q = None.
+        { eapply eval_list_incl_none with u ; eauto.
+          apply List.incl_app ; [now apply List.incl_refl | ].
+          intros x [Hinx | Hinx] ; inversion Hinx.
+          now apply eval_list_In.
+        }
+        econstructor ; [ now apply eval_list_In_is_fun | left].
+        exists q ; split ; [ now auto | split ; [ auto | ] ].
+        intros a'.
+        suff: ext_tree_indbarredP tau (u ++ [::(q, a')]).
+        { intros H ; unshelve eapply (ext_tree_indbarredP_monotone H).
+          + rewrite cats1 ; apply is_fun_rcons_notin_dom.
+            * now apply eval_list_In_is_fun.
+            * now apply eval_list_notin.
+          + apply List.incl_app ; [ | now apply List.incl_appr,List.incl_refl].
+            do 2 apply List.incl_appl ; now apply List.incl_refl.
+        }
+        destruct (@eqP I q i) as [Heqi | Hnoteq] ; [subst | exfalso ].
+        -- apply (Hyp a').
+           rewrite cats1 ; now apply Add_rcons.
+        -- suff: eval_list l q = None by (intros H ; rewrite H in Hsome ; now inversion Hsome).
+           eapply eval_list_incl_none with (u ++ [::(i, o)]).
+           ++ now apply eval_list_none_fun.
+           ++ intros x Hinx ; eapply (List.Add_in Hadd) in Hinx.
+              destruct Hinx as [Hinx | Hinx] ; eapply List.in_or_app ; [| now left].
+              right ; now left.
+           ++ eapply eval_list_notin_cat ; auto ; cbn.
+              intros [Hin | Hin] ; inversion Hin ; now auto.
+    + destruct (@eqP I q' i) as [Heqi | Hnoteq] ; [subst | exfalso ].
+      * econstructor ; [assumption | left].
+        exists i ; split ; [auto | split ; [auto | ] ].
+        intros a ; apply (Hyp a).
+        rewrite cats1 ; now apply Add_rcons.
+      * have auxl : eval_list l q' = None.
+        -- eapply eval_list_incl_none with (u ++ [::(i, o)]).
+           ++ now apply eval_list_none_fun.
+           ++ intros x Hinx ; eapply (List.Add_in Hadd) in Hinx.
+              destruct Hinx as [Hinx | Hinx] ; eapply List.in_or_app ; [| now left].
+              right ; now left.
+           ++ eapply eval_list_notin_cat ; auto ; cbn.
+              intros [Hin | Hin] ; inversion Hin ; now auto.
+        -- suff: ask (R := A) q = ask q' by
+             (intros H ; inversion H ; subst ; rewrite auxl in Hsome ; inversion Hsome).
+           rewrite - Heq.
+           eapply eval_ext_tree_aux_finapp_monotone_ask_list ; eauto.
+           rewrite - addn1 ; now apply eval_ext_tree_aux_finapp_monotone_ask_fuel.
+  - have Hfunu : is_fun_list u.
+    { eapply is_fun_list_incl ; eassumption. } 
+    remember (eval_ext_tree_aux_finapp tau u (size u) nil) as aux.
+    destruct aux as [q' | r].
+    2: econstructor ; [ assumption | right ; left ; now exists r ].
+    remember (eval_list u q') as aux2 ; destruct aux2 as [a | ].
+    + econstructor ; [ assumption | ].
+      right ; right ; exists q',a.
+      split ; [now auto | split ; [now auto | ] ].
+      remember (eval_ext_tree_aux_finapp tau (u ++[:: (q', a)]) (size (u ++ [:: (q', a)])) nil)
+        as aux3.
+      destruct aux3 as [q'' | r].
+      2: econstructor ; [now apply eval_list_In_is_fun | right ; left ; now exists r ].
+      suff: q'' = q.
+      2:{ suff: ask (R := A) q'' = ask q by (intros H ; inversion H).
+          have Heqsize: (size l = (size u).+1) by (eapply List.Add_length ; eassumption).
+          rewrite Heqaux3 - Heq size_cat addn1 Heqsize.
+          eapply eval_ext_tree_aux_finapp_one_step_fuel ; eauto.
+          * now apply eval_list_In_is_fun.
+          * now apply List.incl_appl, List.incl_refl.
+      }
+      intros e ; subst.
+      have Hnone': eval_list (u ++ [:: (q', a)]) q = None.
+      { eapply eval_list_incl_none ; [ | | eassumption ] ; auto.
+        eapply List.incl_tran ; [ | exact Hincl].
+        apply List.incl_app ; [now apply List.incl_refl | ].
+        intros x [Hinx | Hinx] ; inversion Hinx ; now apply eval_list_In.
+      }
+      econstructor ; [now apply eval_list_In_is_fun | left].
+      exists q ; split ; [auto | split ; [auto | ] ].
+      intros o'.
+      suff: ext_tree_indbarredP tau (u ++ [::(q, o')]).
+      { intros H ; unshelve eapply (ext_tree_indbarredP_monotone H).
+        + rewrite cats1 ; apply is_fun_rcons_notin_dom.
+          * now apply eval_list_In_is_fun.
+          * now apply eval_list_notin.
+        + apply List.incl_app ; [ | now apply List.incl_appr,List.incl_refl].
+          do 2 apply List.incl_appl ; now apply List.incl_refl.
+      }
+      have Hnoneu: eval_list (u ++ [:: (q, o')]) i = None.
+      { apply eval_list_notin_cat ; [assumption | ].
+        cbn ; intros [Hfalse | Hfalse] ; [ subst | now inversion Hfalse].
+        suff: eval_list l i = Some o.
+        { intros H ; rewrite H in Hnonel ; now inversion Hnonel. }
+        apply (In_eval_list Hfunl).
+        unshelve eapply (List.Add_in Hadd) ; now left.
+      }
+      eapply (IHk o') ; eauto.
+      -- apply List.incl_app ; [now apply List.incl_appl | ].
+         apply List.incl_appr, List.incl_refl.
+      -- now apply Add_cat.
+      -- intros a' w Haddw.
+         suff: exists x, List.Add (q,o') x w.
+         2:{ eapply List.Add_inv.
+             apply (List.Add_in Haddw) ; right ; apply List.in_or_app.
+             right ; now left.
+         }
+         intros [x Haddx].
+         eapply (ext_tree_indbarredP_monotone) with x.
+         ++ eapply Hyp with a'.
+            eapply (@Add_diamond _ _ _ u (u ++ [:: (q, o')]) x w) ; eauto.
+            rewrite cats1 ; eapply Add_rcons.
+         ++ eapply is_fun_list_incl with ((u ++ [:: (q, o')]) ++ [::(i, a')]).
+            { do 2 (apply eval_list_none_fun ; auto).
+              eapply eval_list_incl_none ; [ | | eassumption ] ;
+                [ now apply eval_list_In_is_fun | ].
+              now apply List.incl_appl, List.incl_refl.
+            }
+            intros y Hiny ; apply (List.Add_in Haddw) in Hiny.
+            destruct Hiny as [Hiny | Hiny] ; [subst | ].
+            ** apply List.in_or_app ; right ; now left.
+            ** apply List.in_or_app ; now left.
+         ++ intros y Hin ; eapply List.Add_in ; [eassumption | now right].
+    + destruct (@eqP I q' i) as [Heqi | Hnoteq] ; [ subst | ].
+      * econstructor ; [assumption | ].
+        left ; exists i ; split ; [auto | split ; [ auto | ] ].
+        intros o' ; apply (Hyp o').
+        rewrite cats1 ; now apply Add_rcons.
+      * suff: q' = q ; [intros Heqq ; subst | ].
+        -- econstructor ; [assumption | ].
+           left ; exists q ; split ; [auto | split ; [ auto | ] ].
+           intros o' ; eapply (IHk o').
+           ++ apply List.incl_app ; [now apply List.incl_appl | ].
+              apply List.incl_appr, List.incl_refl.
+           ++ apply eval_list_notin_cat ; [assumption | ].
+              cbn ; intros [Heqi | Hfalse] ; now auto.
+           ++ now apply Add_cat.
+           ++ intros a w Haddw.
+              eapply ext_tree_indbarredP_monotone with ((i,a) :: u).
+              ** now apply Hyp with a, List.Add_head.
+              ** eapply is_fun_list_incl with ((u ++ [:: (q, o')]) ++ [::(i, a)]).
+                 { apply eval_list_none_fun ; auto ; [ now apply eval_list_none_fun | ].
+                   apply eval_list_notin_cat ; auto ; cbn.
+                   intros [Heqi | Hfalse] ; [now subst | now inversion Hfalse].
+                 }
+                 intros y Hiny ; apply (List.Add_in Haddw) in Hiny.
+                 destruct Hiny as [Hiny | Hiny] ; [subst | ].
+                 --- apply List.in_or_app ; right ; now left.
+                 --- apply List.in_or_app ; now left.
+              ** intros x Hinx.
+                 eapply (List.Add_in Haddw) ; rewrite - cat_cons.
+                 apply List.in_or_app ; now left.
+        -- suff: ask (R := A) q = ask q' by (inversion 1).
+           erewrite <- Heq, List.Add_length ; eauto.
+           eapply eval_ext_tree_aux_finapp_monotone_ask_list ; eauto.
+           ++ eapply eval_list_incl_none with ((i,o) :: u).
+              ** eapply is_fun_cons_notin_dom ; eauto.
+                 now apply eval_list_notin.
+              ** intros x Hinx ; now apply (List.Add_in Hadd) in Hinx.
+              ** cbn ; erewrite ifN_eq ; [now auto | ].
+                 eapply contra_not_neq with (q' = i) ; auto.
+           ++ rewrite - addn1.
+              eapply eval_ext_tree_aux_finapp_monotone_ask_fuel ; eauto.
+Qed.
+
+(*              apply eval_list_In_is_fun ; auto.
+              | ].
+              intros y Hiny ; apply (List.Add_in Haddw) in Hiny.
+              destruct Hiny as [Heqy | Hinu] ; [subst | ].
+              
+           admit.
+      * admit.
+    + suff: q' = i.
+      * intros e ; subst.
+        
+      *
+           apply List.Add_split in Haddw as [w1 [w2 [Heqw1 Heqw2]]] ; subst.
+           suff: ext_tree_indbarredP tau (w1 ++ ((i, a') :: w2)%SEQ)
+           
+           remember (eval_list u i) as test ; destruct test as [a' | ].
+           
+           admit.
+        -- 
+        
+
+        -- suff: o' = o.
+           { intros H ; subst.
+             econstructor ; [admit | ].
+             left.
+             exists q ; split ; [auto | split ; [ auto | ] ].
+             intros o'.
+             suff: ext_tree_indbarredP tau (u ++ [::(q, o')]).
+             { intros H ; unshelve eapply (ext_tree_indbarredP_monotone H).
+               + admit.
+               + apply List.incl_app ; [ | now apply List.incl_appr,List.incl_refl].
+                 do 2 apply List.incl_appl ; now apply List.incl_refl.
+             }
+             apply (Hyp o') ; admit.
+           }
+           suff: List.In (q,o) l.
+           { intros H ; apply (In_eval_list Hfunl) in H ; rewrite H in Hsome.
+             now injection Hsome.
+           }
+           eapply List.Add_in ; [exact Hadd | now left].
+        -- econstructor ; [ admit | left].
+           exists q ; split ; [ now auto | split ; [now auto | ] ].
+           intros a'.
+           suff: 
+           cbn.
+           
+           
+             eapply IHk.
+           
+         2:{
+        
+        
+        
+      * suff: q = q''.
+        { intros Heq' ; subst.
+          specialize (IHk i o u (v ++ [::(q'', o')])).
+          Print List.Add.
+          suff: ext_tree_indbarred
+  - subst.
+    econstructor ; [assumption | ].
+    remember (eval_ext_tree_aux_finapp tau u (size u) [::]) as val.
+    destruct val as [q | r].
+    2:{ right ; left ; eauto. }
+    remember (eval_list u q) as val2 ; destruct val2 as [o' |].
+    + symmetry in Heqval, Heqval2.
+      suff: List.incl u (u ++ [::(i,o)]).
+      * intros Htest.
+        right ; right.
+        exists q, o' ; split ; [auto | split ; [auto | ] ].
+        econstructor.
+        { now apply eval_list_In_is_fun. }
+        right ; left.
+        exists a.
+        revert Heqa.
+        admit.
+      * apply List.incl_appl, List.incl_refl.
+    + left.
+      exists q.
+      split ; [reflexivity | split ; [now auto | ] ].
+      remember (eval_list [::(i,o)] q) as aux ; destruct aux as [o' | ].
+      { cbn in *.
+        destruct (@eqP I q i) as [? | Hnoteq] ; [subst ; assumption | now inversion Heqaux].
+      }
+      symmetry in Heqaux,Heqval,Heqval2 ; apply eval_list_notin in Heqaux.
+      exfalso.
+      eapply (eval_ext_tree_aux_finapp_monotone_ask_fuel 1 Hfun Heqval2) in Heqval.
+      eapply (eval_ext_tree_aux_finapp_monotone_ask_list) in Heqval ; [ | exact Hnodup | | ].
+      * rewrite size_cat Heqval in Heqa ; now inversion Heqa.
+      * now apply List.incl_appl, List.incl_refl.
+      * now apply eval_list_notin_cat.
+  - subst.
+    remember (eval_ext_tree_aux_finapp tau u (size u) nil) as aux.
+    destruct aux as [q' | r].
+    2: econstructor ; [assumption | right ; left ; now exists r ].
+    remember (eval_list u q') as aux2 ; destruct aux2 as [a | ].
+    + econstructor ; [ assumption | ].
+      right ; right ; exists q',a.
+      split ; [now auto | split ; [now auto | ] ].
+      remember (eval_ext_tree_aux_finapp tau (u ++ [:: (q', a)]) (size (u ++ [:: (q', a)])) nil)
+        as aux3.
+      destruct aux3 as [q'' | r].
+      2: econstructor ; [now apply eval_list_In_is_fun | right ; left ; now exists r ].
+      remember (eval_list (u ++ [:: (q', a)]) q'') as aux4 ; destruct aux4 as [a' | ].
+      * suff: q = q''.
+        { intros Heq' ; subst.
+          specialize (IHk i o (u ++ [::(q'', o')])).
+          suff: ext_tree_indbarred
+          
+      
+      unshelve eapply IHk.
+      
+
+      
+    specialize (IHk q o' (u ++ [::(i, o)])).
+*)
+    
+  
+Lemma test (tau : ext_tree) (l : seq (I * O)) (o : O) :
+  indbarred_fun_list
+    (fun u => exists n a, eval_ext_tree_aux_finapp tau u n nil = output a) l ->
+  ext_tree_indbarredP tau l.
+Proof.
+  intros Hyp.
+  assert (aux := indbarred_fun_list_fun_list Hyp) ; revert aux.
+  induction Hyp as [u v [n [r Hr]] Hincl Hnodup | q v Hnotin _ IHk].
+  - intros Hfun ; eapply eval_output_indbarredP ; eauto.
+    eapply eval_ext_tree_aux_finapp_monotone_output_list ; now eauto.
+  - intros Hfun.
+    unshelve eapply super with (v ++ [::(q,o)]) q o.
+    + rewrite - (cat0s v) ; apply eval_list_notin_cat; auto.
+    + rewrite cats1 ; now apply Add_rcons.
+    + apply IHk.
+      rewrite cats1.
+      now apply is_fun_rcons_notin_dom.
+    + intros o' w Haddw.
+      suff: List.incl (v ++ [:: (q, o')]) w.
+      { intros Hincl.
+        eapply ext_tree_indbarredP_monotone ; [ apply IHk | | eassumption].
+        * rewrite cats1.
+          now apply is_fun_rcons_notin_dom.
+        * apply is_fun_list_incl with (v ++ [::(q, o')]).
+          -- rewrite cats1 ; now apply is_fun_rcons_notin_dom.
+          -- intros x Hinx ; apply (List.Add_in Haddw) in Hinx.
+             destruct Hinx as [Hinx | Hinx] ; [subst | ] ; apply List.in_or_app ; auto.
+             now right ; left.
+      }
+      intros x Hinx ; apply (List.Add_in Haddw).
+      apply List.in_app_or in Hinx ; destruct Hinx as [Hinx | Hinx] ; [now right | ].
+      destruct Hinx ; now left.
+Qed.
+
+Lemma test_noo (tau : ext_tree) (l : seq (I * O)) :
+  indbarred_fun_list
+    (fun u => exists n a, eval_ext_tree_aux_finapp tau u n nil = output a) l ->
+  ext_tree_indbarredP tau l.
+Proof.
+  destruct l as [ | [i o] l] ; intros Hyp.
+  - econstructor ; [intros i j K H ; inversion H | cbn ].
+    remember (tau nil) as aux ; destruct aux as [q | r] ; [ | right ; left ; now exists r].
+    left ; exists q ; split ; [auto | split ; [auto | ] ].
+    intros o.
+    eapply ext_tree_indbarredP_monotone with nil.
+    + now eapply test.
+    + intros i a a' Hina Hina'.
+      destruct Hina as [H | H] ; inversion H ; subst ; clear H.
+      destruct Hina' as [H | H] ; inversion H ; now subst.
+    + now apply List.incl_nil_l.
+  - eapply test ; eauto.
+Qed.
+  
+  
+
+  
+Lemma eval_ext_tree_finapp_trace (tau : ext_tree) f n a l :
+  eval_ext_tree_aux tau f n l = output a ->
+  eval_ext_tree_aux_finapp tau [seq (i, f i) | i <- eval_ext_tree_trace_aux tau f n l]
+    (size (eval_ext_tree_trace_aux tau f n l)) l = output a.
+Proof.
+  assert (aux := @is_fun_map (eval_ext_tree_trace_aux tau f n l) f) ; revert aux.
+  change (eval_ext_tree_trace_aux tau f n l) with (nil ++ (eval_ext_tree_trace_aux tau f n l)) at 1 2.
+  generalize (@nil I) as u ; revert l.
+  induction n as [ | n IHn] ; cbn in * ; intros l u aux Heq.
+  { destruct u ; cbn ; [assumption | now rewrite Heq ]. }
+  remember (tau l) as r ; destruct r ; cbn in *.
+  2:{ destruct u ; cbn ; now rewrite - Heqr. }
+  erewrite <- cat_rcons, <- Heqr ; rewrite - cat_rcons in aux.
+  suff: eval_list [seq (i, f i) | i <- rcons u s ++ eval_ext_tree_trace_aux tau f n (rcons l (f s))] s = Some (f s).
+  { intros Hyp ; rewrite Hyp.
+    specialize (IHn (rcons l (f s)) (rcons u s)) ; erewrite IHn ; [reflexivity | assumption | assumption].
+  }
+Admitted.
+Print deval.
+
+Fixpoint deval_list (d : @dialogue I O A) (l : list (I * O)) : option A :=
+  match d with
+  | eta a => Some a
+  | beta q k => match eval_list l q with
+                | None => None
+                | Some o => deval_list (k o) l
+                end
+  end.
+
+Lemma deval_list_deval d l alpha a:
+  deval_list d [seq (i, alpha i) | i <- l] = Some a ->
+  deval d alpha = a.
+Admitted.
+
+Fixpoint deval_trace (d : @dialogue I O A) f : list (I * O) :=
+  match d with
+  | eta a => nil
+  | beta q k => (q, (f q)) :: (deval_trace (k (f q)) f)
+  end.
+
+
+  
+Theorem GBI_GCI F :
+  seq_cont_valid F ->
+  dialogue_cont F.
+Proof.
+  intros [tau [HF Hval]].
+  eapply Delta0_choice in HF as [HF].
+  2:{
+    intros α n. destruct eval_ext_tree eqn:E.
+    - firstorder congruence.
+    - left. destruct (HF α) as [m].
+      f_equal. 
+      eapply eval_ext_tree_output_unique; eauto. 
+  }
+  unfold GBI in HGBI.
+  pose (T := fun (l : list (I * O)) =>
+               exists d : dialogue,
+                 forall (l' : list (I * O)) (a : A),
+                   List.incl l l' ->
+                    deval_list d l' = Some a <->
+                      eval_ext_tree_aux_finapp tau l' (size l') nil = output a).
+  have Help : ABbarred T.
+  { intros alpha.
+    destruct (HF alpha) as [n Hn].
+    exists (eval_ext_tree_trace tau alpha n).
+    unfold T.
+    exists (eta (F alpha)).
+    intros l' a Hincl.
+    split ; intros Hyp.
+    + cbn in *.
+      inversion Hyp ; subst ; clear Hyp.
+      admit.
+    + cbn in *.
+      admit.
+  }
+  apply HGBI, indbarred_indbarred_NoDup in Help.
+  unfold dialogue_cont.
+  unfold T in * ; clear T.
+  suff: exists d : dialogue, forall (l : list (I * O)) (a : A),
+      List.incl nil l ->
+      deval_list d l = Some a <->
+      eval_ext_tree_aux_finapp tau l (size l) nil = output a.
+
+  { intros [d Hd].
+    exists d ; intros alpha.
+    specialize (HF alpha) as [n Hn].
+    specialize (Hd [seq (i, alpha i) | i <- eval_ext_tree_trace tau alpha n] (F alpha))
+      as [Hd1 Hd2] ; [now apply List.incl_nil_l | ].
+    suff: deval_list d [seq (i, alpha i) | i <- eval_ext_tree_trace tau alpha n] = Some (F alpha).
+    { intros Hyp.
+      symmetry ; eapply deval_list_deval.
+      eassumption.
+    }
+    apply Hd2 ; rewrite size_map.
+    apply eval_ext_tree_finapp_trace ; exact Hn.
+  }
+  revert Help ; clear HF F.
+  generalize (@nil (I * O)).
+  intros l Help.
+  pattern l.
+  induction Help.
+  - destruct H as [d Hd].
+    exists d.
+    intros l' a Hincl.
+    assert (Hincl' := List.incl_tran H0 Hincl).
+    specialize (Hd l' a Hincl') as [Hd1 Hd2] ; split ; intros Hyp.
+    + now apply Hd1.
+    + now apply Hd2.
+  - clear H0.
+    
+    
+    
+    exists d.
+    intros
+  
+  
+  
+  induction Help.
+  
+  
+    
+    2:{ cbn.
+
+  
+  pose (T := fun (l : list (I * O)) =>
+               forall l', List.incl l l' ->
+                          List.NoDup (map fst l') ->
+                          exists a : A,
+                            eval_ext_tree_aux_finapp tau l' (size l') (map snd l) = output a).
+  have Help : ABbarred T.
+  { intros alpha.
+    destruct (HF alpha) as [n Hn].
+    exists (eval_ext_tree_trace tau alpha n).
+    unfold T.
+    intros l' Hincl Hnodup ; exists (F alpha).
+    admit.
+  }
+  apply HGBI, indbarred_indbarred_NoDup in Help.
+  unfold dialogue_cont.
+  
+  induction Help.
+
+  
+  unfold T in * ; clear T.
+  suff: exists d : dialogue, forall alpha : I -> O,
+    exists l : seq (I * O),
+      map alpha (map fst l) = map snd l /\
+        forall l',
+          List.incl l l' ->
+          List.NoDup (map fst l') ->
+          eval_ext_tree_aux_finapp tau l' (size l') (map snd l) = output (deval d alpha).
+  {admit. }
+
+  
+  revert Help HF.
+  unfold eval_ext_tree.
+
+  
+  change (@nil O) with (map snd (@nil (I * O))).
+  generalize (@nil (I * O)) ; intros l Help.
+  pattern l ; induction Help as [u v Hv Hincl Hnodup | ] ; intros HF.
+  - specialize (Hv u Hincl Hnodup) as [a Ha].
+    exists (eta a).
+    intros alpha ; cbn.
+    specialize (HF alpha) as [n Hn].
+    exists v.
+    
+    suff: output (Q := I) (F alpha) = output a by (intros Heq ; inversion Heq).
+    rewrite - Ha ; symmetry.
+    
+
+  
+  suff: exists d : dialogue, forall (alpha : I -> O),
+    exists l, (map alpha (map fst l)) = map snd l /\
+                eval_ext_tree_aux_finapp tau l (size l) nil = output (deval d alpha).
+  { intros [d Hd].
+    exists d.
+    intros alpha.
+    specialize (Hd alpha) as [l [Hl1 Hl2]].
+    admit. }
+  clear HF.
+  have aux: forall alpha, map alpha (map fst (@nil (I * O))) = map snd (@nil (I * O))
+      by reflexivity.
+  revert Help aux.
+  generalize (@nil (I * O)).
+  intros l Help ; pattern l ; induction Help as [u v Hv Hincl Hnodup | ] ; intros aux.
+  - destruct Hv as [a Ha] ; exists (eta a).
+    intros alpha ; cbn ; exists v.
+    split.
+    { admit. }
+    assumption.
+  -
+
+  
+  - revert Hv u Hincl Hnodup.
+    generalize 0 as m.
+    induction v as [ | v x] using last_ind ; intros.
+    { cbn in *.
+      destruct Hv as [a Heqa].
+      exists (eta a) ; intros alpha.
+      exists nil ; cbn.
+      change (map snd u) with (map snd (nil ++ u)) ; rewrite map_cat.
+      now erewrite valid_cat. 
+    }
+    cbn in *.
+(*    remember (tau (map snd u)) as r.
+    destruct r as [ i | ].
+    2:{ exists (eta a) ; intros alpha ; exists 1.
+        cbn ; now rewrite <- Heqr. }
+    cbn in Hv.*)
+    rewrite size_rcons in Hv; cbn in *.
+    remember ( tau [seq i.2 | i <- take m (rcons v x)]) as s.
+    destruct s as [j | a].
+
+    2:{ exfalso.
+        erewrite valid_cat in Heqr.
+        
+    
+
+
+
+
+
+
+
+
+
+
+
+  
+  suff: exists d : dialogue, forall alpha : I -> O,
+      eval_ext_tree_aux_finapp tau (deval_trace d alpha) (size (deval_trace d alpha)) nil =
+        output (deval d alpha).
+  { admit. }
+  clear HF ; unfold T in * ; clear T.
+  revert Help.
+  generalize (@nil (I * O)) ; generalize 0 ; intros n l Help.
+  pattern l.
+  induction Help as [u v [a Ha] Hincl Hnodup | i v Hnotin _ IHk].
+  {
+  2:{
+
+
+    unfold T in *.
+     
+
+  
+  unfold T in * ; clear T.
+  suff: exists d : dialogue, forall (l : list (I * O)) (a : A),
+      deval_list d l = Some a <->
+      eval_ext_tree_aux_finapp tau l (size l) nil = output a.
+
+  { intros [d Hd].
+    exists d ; intros alpha.
+    specialize (HF alpha) as [n Hn].
+    specialize (Hd [seq (i, alpha i) | i <- eval_ext_tree_trace tau alpha n] (F alpha))
+      as [Hd1 Hd2].
+    suff: deval_list d [seq (i, alpha i) | i <- eval_ext_tree_trace tau alpha n] = Some (F alpha).
+    { intros Hyp.
+      symmetry ; eapply deval_list_deval.
+      eassumption.
+    }
+    apply Hd2 ; rewrite size_map.
+    apply eval_ext_tree_finapp_trace ; exact Hn.
+  }
+  clear HF.
+  revert Help.
+  replace (@nil O) with (map snd (take 0 (@nil (I * O)))) by reflexivity.
+  generalize (@nil (I * O)) ; generalize 0 ; intros n l Help.
+  pattern l.
+  induction Help as [u v [a Ha] Hincl Hnodup | i v Hnotin _ IHk].  
+  - admit.
+  - 
+
+    exists (eta a).
+    intros w a'.
+    split ; cbn.
+    { intros Heq ; inversion Heq ; subst.
+      
+    exists (size v) ; cbn.
+    rewrite - Ha.
+
+
+  
+    eapply eval_ext_tree_output_unique ; [eassumption | ].
+    
+    
+      exists n, eval_ext_tree_aux tau alpha n (take 0 nil) = output (deval d alpha).
+  { intros [d Hd].
+    exists d ; intros alpha ; specialize (Hd alpha) as [n Hn] ; [ reflexivity | ].
+    specialize (HF alpha) as [m Hm] ; unfold eval_ext_tree in *.
+    eapply eval_ext_tree_output_unique ; eassumption.
+  }
+  clear HF.
+  revert Help.
+  replace (@nil O) with (map snd (@nil (I * O))) ; change (@nil I) with (map fst (@nil (I * O))).
+  generalize (@nil (I * O)) ; generalize 0 ; intros n l Help.
+  pattern l.
+  induction Help as [u v [a Ha] Hincl Hnodup | i v Hnotin _ IHk].  
+  - exists (eta a).
+    intros alpha Heqalpha.
+    exists (size v) ; cbn.
+    rewrite - Ha.
+    
+
+    revert Hv u Hincl Hnodup.
+    replace (@nil O) with (take 0 (map snd v)) by (now rewrite take0).
+    clear T ; generalize 0 as m.
+    induction v as [ | x] ; intros.
+    { cbn in *.
+      destruct Hv as [a Heqa].
+      exists (eta a) ; intros alpha ; exists 1 ; cbn.
+      unfold valid_ext_tree in Hval.
+      change (map snd u) with (map snd (nil ++ u)) ; rewrite map_cat.
+      now erewrite valid_cat. 
+    }
+    remember (tau (map snd u)) as r.
+    destruct r as [ i | ].
+    2:{ exists (eta a) ; intros alpha ; exists 1.
+        cbn ; now rewrite <- Heqr. }
+    cbn in Hv.
+    remember (tau (take m (x.2 :: [seq i.2 | i <- v]))) as s.
+    destruct s as [j | a].
+    2:{ exfalso.
+        erewrite valid_cat in Heqr.
+        
+
+
+
+
+
+
+
+
+
+
+  
+  
+  pose (T := fun (l : list (I * O)) =>
+               (exists a : A, forall f, map f (map fst l) = map snd l ->
+                                        eval_ext_tree_aux tau f (size l) nil = output a)).
+  have Help : ABbarred T.
+  { intros alpha.
+    destruct (HF alpha) as [n Hn].
+    exists (eval_ext_tree_trace tau alpha n).
+    unfold T.
+    exists (F alpha) ; intros f.
+    erewrite <- (map_comp fst _).
+    erewrite (@eq_map _ _ (fst \o (fun i : I => (i, alpha i))) id) ; [ | now intros k].
+    erewrite map_id, <- (map_comp snd _).
+    erewrite (@eq_map _ _ (snd \o (fun i : I => (i, alpha i))) alpha) ; [ | now intros k].
+    intros Heqf.
+    assert (aux:= eval_ext_tree_trace_size_eval_trace Hn).
+    apply eval_ext_tree_trace_size_eval in Hn ; rewrite <- Hn, size_map ; symmetry.
+    apply eval_ext_tree_continuous.
+    now rewrite - aux.
+  }
+  apply HGBI, indbarred_indbarred_NoDup in Help.
+  unfold dialogue_cont.
+  eapply Delta0_choice in HF as [HF].
+  2:{
+    intros α n. destruct eval_ext_tree eqn:E.
+    - firstorder congruence.
+    - left. destruct (HF α) as [m].
+      f_equal. 
+      eapply eval_ext_tree_output_unique; eauto. 
+  }
+  unfold T in * ; clear T.
+  suff: exists d : dialogue, forall (alpha : I -> O),
+    exists n, eval_ext_tree_aux tau alpha n nil = output (deval d alpha).
+  { intros [d Hd].
+    exists d ; intros alpha ; specialize (Hd alpha) as [n Hn].
+    specialize (HF alpha) as [m Hm] ; unfold eval_ext_tree in *.
+    eapply eval_ext_tree_output_unique ; eassumption.
+  }
+  clear HF.
+  revert Help ; unfold inductively_barred, eval_ext_tree.
+  have aux : forall (f : I -> O), [seq f i | i <- [seq i.1 | i <- (@nil (I * O))]] =
+                                    [seq i.2 | i <- (@nil (I * O))].
+  intros f ; reflexivity.
+  revert aux.
+  generalize (@nil (I * O)) ; intros l Hyp Help ; revert Hyp.
+  pattern l.
+  induction Help as [u v Hv Hincl Hnodup | i v Hnotin _ IHk] ; intros Hyp.
+  
+  - destruct Hv as [a Ha].
+    exists (eta a) ; intros alpha ; exists (size v).
+    cbn.
+    apply Ha.
+    admit.
+  -
+    
+  
+
+
+
+
+  
+  
+  pose (gs := @eval_ext_tree_continuous _ _ _ tau) ; unfold modulus in gs.
+    
+               exists a : A, eval_ext_tree_aux_finapp tau l (size l) nil = output a).
+  have Help : ABbarred T.
+  { intros alpha.
+    destruct (HF alpha) as [n Hn].
+    exists (eval_ext_tree_trace tau alpha n).
+    unfold T.
+    exists (F alpha).
+    rewrite - Hn size_map.
+
+    
+
+  
+    
+    admit.
+  }
+(*    exists (F alpha).
+    rewrite - Hn eval_ext_tree_map.
+    f_equal.
+    erewrite <- map_comp ; apply eq_map.
+    intros i ; reflexivity.
+ *)
+  apply HGBI, indbarred_indbarred_NoDup in Help.
+  unfold dialogue_cont.
+  eapply Delta0_choice in HF as [HF].
+  2:{
+    intros α n. destruct eval_ext_tree eqn:E.
+    - firstorder congruence.
+    - left. destruct (HF α) as [m].
+      f_equal. 
+      eapply eval_ext_tree_output_unique; eauto. 
+  }
+  unfold T in * ; clear T.
+  suff: exists d : dialogue, forall (alpha : I -> O),
+    exists l, eval_ext_tree_aux_finapp tau l (size l) nil = output (deval d alpha).
+  { admit. }
+  
+  
+  
+  { intros [b Hb].
+    exists b ; intros alpha; specialize (Hb alpha) as [n Heqn].
+    specialize (HF alpha) as [m Heqm].
+    unfold eval_ext_tree in *.
+    eapply eval_ext_tree_output_unique ; eassumption.
+  }
+  revert Help HF ; unfold inductively_barred, eval_ext_tree.
+  change (@nil O) with (map snd (@nil (I * O))).
+  generalize (@nil (I * O)) ; intros l Help HF.
+
+  clear HF.
+  pattern l.
+  induction Help as [u v Hv Hincl Hnodup | ].
+  - unfold T in Hv.
+    revert Hv u Hincl Hnodup.
+    replace (@nil O) with (take 0 (map snd v)) by (now rewrite take0).
+    clear T ; generalize 0 as m.
+    induction v as [ | x] ; intros.
+    { cbn in *.
+      destruct Hv as [a Heqa].
+      exists (eta a) ; intros alpha ; exists 1 ; cbn.
+      unfold valid_ext_tree in Hval.
+      change (map snd u) with (map snd (nil ++ u)) ; rewrite map_cat.
+      now erewrite valid_cat. 
+    }
+    remember (tau (map snd u)) as r.
+    destruct r as [ i | ].
+    2:{ exists (eta a) ; intros alpha ; exists 1.
+        cbn ; now rewrite <- Heqr. }
+    cbn in Hv.
+    remember (tau (take m (x.2 :: [seq i.2 | i <- v]))) as s.
+    destruct s as [j | a].
+    2:{ exfalso.
+        erewrite valid_cat in Heqr.
+        
+    
+    
+    cbn in *.
+
+      
+
+    unfold T ; intros u ; destruct (tau u) ; [left ; now exists a | right].
+    intros [a Hyp] ; now inversion Hyp.
+  - clear l Help.
+    intros u Hu ; cbn.
+    remember (tau u) as r ; destruct r.
+    + exists (spit a) ; intros alpha ; exists 0 ; now cbn.
+    + exfalso ; destruct Hu as [a Ha] ; rewrite Ha in Heqr.
+      now inversion Heqr.
+  - intros u k IHk ; cbn in *.
+    unshelve eexists.
+    + apply bite ; intros o.
+      exact (proj1_sig (IHk o)).
+    + cbn.
+      intros alpha.
+      destruct (IHk (alpha 0)) as [b IHb].
+      destruct (IHb (alpha \o succn)) as [n Hn] ; cbn in *.
+      exists (S n) ; cbn ; rewrite <- Hn.
+      clear -Hvalid.
+      remember (tau u) as r ; destruct r.
+      * destruct n ; cbn ; [symmetry ; now apply Hvalid |].
+        suff: tau (rcons u (alpha 0)) = Some a by (intros Hyp ; now rewrite Hyp).
+        now apply Hvalid.
+      * generalize 0 ; clear Heqr ; revert alpha u.
+        induction n ; [ reflexivity | cbn ; intros alpha u i].
+        destruct (tau (rcons u (alpha i))) ; [reflexivity |].
+        now eapply IHn.
+Qed.
+  
+  
+End GeneralisedBarInduction.
